working loop rule

src/Self.hs
@@ -1,0 +1,14 @@
+module Self where
+
+data Var deriving (Show, Read, Eq, Ord)
+data AExpr deriving (Show, Read, Eq, Ord)
+data BExpr deriving (Show, Read, Eq, Ord)
+
+data Com
+  = Assign Var AExpr
+  | Assert BExpr
+  | Seq Com Com
+  | Sum Com Com
+  | Prod Com Com
+  | Loop Com
+  deriving (Show, Read, Eq, Ord)
